CC/Sep/Basic.lean
@@ -15,8 +15,8 @@ lemma Sep.subcapt_pres_motive (Γ : Ctx n m) (C1 C2 : CaptureSet n) : Prop :=
 
 lemma Sep.elem_inv_motive (Γ : Ctx n m) (C1 C2 : CaptureSet n) : Prop :=
   (∀ x, x ∈ C1 -> Sep Γ {x} C2) ∧
-  Sep Γ C1.rdrSet C2 ∧
-  Sep Γ C1.capSet C2
+  (C1.hasRdr -> Sep Γ rdr C2) ∧
+  (C1.hasCap -> Sep Γ cap C2)
 
 lemma Sep.elem_inv' (h : Sep Γ C1 C2) :
   elem_inv_motive Γ C1 C2 ∧ elem_inv_motive Γ C2 C1 := by
@@ -33,94 +33,100 @@ lemma Sep.elem_inv' (h : Sep Γ C1 C2) :
           have h1 := ihs y hy
           have ⟨_, ⟨h2, _⟩⟩ := h1
           apply symm; aesop
-        · let ⟨_, h1, _⟩ := ihr
+        · intros hr
+          let ⟨_, h1, _⟩ := ihr hr
           apply symm; aesop
-        · let ⟨_, h1, _⟩ := ihc
+        · intros hc
+          let ⟨_, h1, _⟩ := ihc hc
           apply symm; aesop
-      · apply symm; apply set
+      · intros hr; apply symm; apply set
         · intros y hy
           have h1 := ihs y hy
           have ⟨_, _, h2, _⟩ := h1
           apply symm; aesop
-        · let ⟨_, _, h1, _⟩ := ihr
+        · intros hr; let ⟨_, _, h1, _⟩ := ihr hr
           apply symm; aesop
-        · let ⟨_, _, h1, _⟩ := ihc
+        · intros hc; let ⟨_, _, h1, _⟩ := ihc hc
           apply symm; aesop
-      · apply symm; apply set
+      · intros hc; apply symm; apply set
         · intros y hy
           have h1 := ihs y hy
           have ⟨_, _, _, h2⟩ := h1
           apply symm; aesop
-        · let ⟨_, _, _, h1⟩ := ihr
+        · intros hr; let ⟨_, _, _, h1⟩ := ihr hr
           apply symm; aesop
-        · let ⟨_, _, _, h1⟩ := ihc
+        · intros hc; let ⟨_, _, _, h1⟩ := ihc hc
           apply symm; aesop
   case degree =>
     apply And.intro
     · apply And.intro <;> try apply And.intro
       · intros x hx
         simp at hx; subst_vars; apply degree <;> aesop
-      · simp; apply empty
-      · simp; apply empty
+      · intros h; exfalso; apply CaptureSet.singleton_hasRdr_absurd h
+      · intros h; exfalso; apply CaptureSet.singleton_hasCap_absurd h
     · apply And.intro <;> try apply And.intro
       · intros x hx
         simp at hx; subst_vars; apply symm; apply degree <;> trivial
-      · simp; apply empty
-      · simp; apply empty
+      · intros h; exfalso; apply CaptureSet.singleton_hasRdr_absurd h
+      · intros h; exfalso; apply CaptureSet.singleton_hasCap_absurd h
   case var hb hsep ih =>
     apply And.intro
     · apply And.intro <;> try apply And.intro
       · intros x hx
         simp at hx; subst_vars; apply var <;> trivial
-      · simp; apply empty
-      · simp; apply empty
+      · intros h; exfalso; apply CaptureSet.singleton_hasRdr_absurd h
+      · intros h; exfalso; apply CaptureSet.singleton_hasCap_absurd h
     · apply And.intro <;> try apply And.intro
       · intros x hx
         apply symm; apply var; trivial
         apply symm; aesop
-      · apply symm; apply var; trivial
+      · intros hr; apply symm; apply var; trivial
         apply symm; aesop
-      · apply symm; apply var; trivial
+      · intros hr; apply symm; apply var; trivial
         apply symm; aesop 
   case reader =>
     apply And.intro
     · apply And.intro <;> try apply And.intro
       · intros x hx
         simp at hx; subst_vars; apply reader <;> trivial
-      · simp; apply empty
-      · simp; apply empty
+      · intros h; exfalso; apply CaptureSet.singleton_hasRdr_absurd h
+      · intros h; exfalso; apply CaptureSet.singleton_hasCap_absurd h
     · apply And.intro <;> try apply And.intro
       · intros x hx
         simp at hx; subst_vars; apply symm; apply reader <;> trivial
-      · simp; apply empty
-      · simp; apply empty
-  case empty =>
+      · intros h; exfalso; apply CaptureSet.singleton_hasRdr_absurd h
+      · intros h; exfalso; apply CaptureSet.singleton_hasCap_absurd h
+  case degree_uniq =>
     apply And.intro
     · apply And.intro <;> try apply And.intro
-      · intros x hx; cases hx
-      · simp; apply empty
-      · simp; apply empty
-    · apply And.intro <;> try apply And.intro <;> try (solve | apply symm; apply empty)
-      intros x _; apply symm; apply empty
+      · intros x hx
+        simp at hx; subst_vars; apply degree_uniq <;> trivial
+      · intros h; exfalso; apply CaptureSet.singleton_hasRdr_absurd h
+      · intros h; exfalso; apply CaptureSet.singleton_hasCap_absurd h
+    · apply And.intro <;> try apply And.intro
+      · intros x hx
+        simp at hx; subst_vars; apply symm; apply degree_uniq <;> trivial
+      · intros h; exfalso; apply CaptureSet.singleton_hasRdr_absurd h
+      · intros h; exfalso; apply CaptureSet.singleton_hasCap_absurd h
 
 lemma Sep.elems_inv (h : Sep Γ C1 C2) (he : x ∈ C1) : Sep Γ {x} C2 := by
   have h0 := Sep.elem_inv' h
   unfold elem_inv_motive at h0
   aesop
 
-lemma Sep.rdr_elem_inv (h : Sep Γ C1 C2) : Sep Γ C1.rdrSet C2 := by
+lemma Sep.rdr_elem_inv (h : Sep Γ C1 C2) : C1.hasRdr -> Sep Γ rdr C2 := by
   have h0 := Sep.elem_inv' h
   unfold elem_inv_motive at h0
   aesop
 
-lemma Sep.cap_elem_inv (h : Sep Γ C1 C2) : Sep Γ C1.capSet C2 := by
+lemma Sep.cap_elem_inv (h : Sep Γ C1 C2) : C1.hasCap -> Sep Γ cap C2 := by
   have h0 := Sep.elem_inv' h
   unfold elem_inv_motive at h0
   aesop
 
 def Sep.narrow_cap_motive (Γ : Ctx n m) (C1 C2 : CaptureSet n) : Prop :=
-  (C1 = { elems := {}, cap := true, rdr := false } → ∀ C, Sep Γ C C2) ∧
-  (C2 = { elems := {}, cap := true, rdr := false } → ∀ C, Sep Γ C1 C)
+  (C1 = cap → ∀ C, Sep Γ C C2) ∧
+  (C2 = cap → ∀ C, Sep Γ C1 C)
 
 lemma Sep.narrow_cap'
   (h : Sep Γ C1 C2) : narrow_cap_motive Γ C1 C2 := by
@@ -129,11 +135,10 @@ lemma Sep.narrow_cap'
   case set ihs ihr ihc =>
     apply And.intro
     · intros he C; subst_vars
-      have ⟨ih, _⟩ := ihc
+      have ⟨ih, _⟩ := ihc cap_hasCap
       apply ih; rfl  
     · intros he C
       apply set <;> aesop
-  case empty => apply And.intro <;> (intros he C; (solve | cases he | apply empty))
   case var hb hsep ih =>
     apply And.intro <;> intros he C
     · rw [CaptureSet.singleton_def'] at he
@@ -147,14 +152,14 @@ lemma Sep.narrow_cap'
     apply And.intro <;> (intros he C; exfalso; apply CaptureSet.singleton_eq_empty_absurd he)
 
 lemma Sep.narrow_cap
-  (h : Sep Γ { elems := {}, rdr := false, cap := true} C2) :
+  (h : Sep Γ cap C2) :
   Sep Γ C1 C2 := by
   have h := Sep.narrow_cap' h; unfold narrow_cap_motive at h
   aesop
 
 lemma Sep.rdr_spec_motive (Γ : Ctx n m) (C1 C2 : CaptureSet n) : Prop :=
-  (C1 = { elems := {}, rdr := true, cap := false } → ∀ x D C S, BoundVar Γ x D (CType.capt C S) → IsReader Γ S → Sep Γ {x} C2) ∧
-  (C2 = { elems := {}, rdr := true, cap := false } → ∀ x D C S, BoundVar Γ x D (CType.capt C S) → IsReader Γ S → Sep Γ C1 {x})
+  (C1 = rdr → ∀ x D C S, BoundVar Γ x D (CType.capt C S) → IsReader Γ S → Sep Γ {x} C2) ∧
+  (C2 = rdr → ∀ x D C S, BoundVar Γ x D (CType.capt C S) → IsReader Γ S → Sep Γ C1 {x})
 
 lemma Sep.rdr_spec' (h : Sep Γ C1 C2) : rdr_spec_motive Γ C1 C2 := by
   induction h <;> unfold rdr_spec_motive at *
@@ -162,8 +167,8 @@ lemma Sep.rdr_spec' (h : Sep Γ C1 C2) : rdr_spec_motive Γ C1 C2 := by
   case set ihs ihr ihc => 
     apply And.intro
     · intros he x D C S hb hr; subst_vars
-      have ⟨ih, _⟩ := ihr
-      apply ih <;> aesop
+      have ⟨ih, _⟩ := ihr rdr_hasRdr
+      apply ih <;> trivial
     · intros he x D C S hb hr
       apply set
       · intros y hy
@@ -171,9 +176,6 @@ lemma Sep.rdr_spec' (h : Sep Γ C1 C2) : rdr_spec_motive Γ C1 C2 := by
         apply h1 <;> trivial
       · aesop
       · aesop
-  case empty => 
-    apply And.intro <;> try (solve | intros he; cases he)
-    intros; apply empty
   case var ih =>
     apply And.intro <;> intros he x D C S hb hr
     · exfalso; apply CaptureSet.singleton_eq_empty_absurd he
@@ -184,7 +186,7 @@ lemma Sep.rdr_spec' (h : Sep Γ C1 C2) : rdr_spec_motive Γ C1 C2 := by
     apply And.intro <;> (intros he C; exfalso; apply CaptureSet.singleton_eq_empty_absurd he)
 
 lemma Sep.rdr_spec
-  (h : Sep Γ { elems := {}, rdr := true, cap := false } C2)
+  (h : Sep Γ rdr C2)
   (hb : BoundVar Γ x D (CType.capt C S))
   (hr : IsReader Γ S) :
   Sep Γ {x} C2 := by
@@ -195,8 +197,8 @@ lemma Sep.subcapt_pres (h : Sep Γ C1 C2) (hsub : Subcapt Γ C0 C1) : Sep Γ C0 
   induction hsub
   case sc_trans ih1 ih2 => aesop
   case sc_elem h => apply Sep.elems_inv <;> trivial
-  case sc_elem_rdr => apply Sep.rdr_elem_inv h
-  case sc_elem_cap => apply Sep.cap_elem_inv h
+  case sc_elem_rdr => apply Sep.rdr_elem_inv h; trivial
+  case sc_elem_cap => apply Sep.cap_elem_inv h; trivial
   case sc_var h => apply var <;> trivial
   case sc_set ihs ihr ihc => apply set <;> aesop
   case sc_rdr_cap => apply narrow_cap h
