CC/Subcapt.lean
@@ -24,20 +24,22 @@ inductive Subcapt : Ctx n m -> CaptureSet n -> CaptureSet n -> Prop where
   x ∈ C ->
   Subcapt Γ {x} C
 | sc_elem_rdr :
-  Subcapt Γ { elems := {}, rdr := brdr, cap := false } { elems := C, rdr := brdr, cap := bcap }
+  C.hasRdr ->
+  Subcapt Γ rdr C
 | sc_elem_cap :
-  Subcapt Γ { elems := {}, rdr := false, cap := bcap } { elems := C, rdr := brdr, cap := bcap }
+  C.hasCap ->
+  Subcapt Γ cap C
 | sc_var :
   BoundVar Γ x D (CType.capt C S) ->
   Subcapt Γ {x} C
 | sc_set :
   (∀ x, x ∈ C1 -> Subcapt Γ {x} C2) ->
-  Subcapt Γ C1.rdrSet C2 ->
-  Subcapt Γ C1.capSet C2 ->
+  (C1.hasRdr -> Subcapt Γ rdr C2) ->
+  (C1.hasCap -> Subcapt Γ cap C2) ->
   Subcapt Γ C1 C2
 | sc_rdr_cap :
-  Subcapt Γ { elems := {}, rdr := true, cap := false } { elems := {}, rdr := false, cap := true }
+  Subcapt Γ rdr cap
 | sc_reader :
   BoundVar Γ x D (CType.capt C S) ->
   IsReader Γ S ->
-  Subcapt Γ {x} { elems := {}, rdr := true, cap := false }
+  Subcapt Γ {x} rdr
